nola/examples/logic/synty.v
@@ -94,4 +94,3 @@ Next Obligation. by move=> ? /of_nsynty_inhab. Qed.
 Next Obligation. by move=> ? /to_nsynty_inhab. Qed.
 
 Notation proph_asnn := (proph_asn nsynty).
-Notation prophn A := (proph nsynty A).
